---
layout: post
title: "数学笔记 - 求导公式"
subtitle: "考研中常用的一些求导公式"
date: 2018-09-09 13:39
author: "Oscaner"
header-img: "img/post-bg-alitrip.jpg"
multilingual: false
mathjax: true
no-catalog: true
categories:
  - skill
  - math
tags:
  - Skill
  - Math
  - Graduate
---

$$
\begin{align*}

  ( c )^\prime &= 0

  \\

  ( x^a )^\prime &= ax^{a - 1}

  \\

  ( \log_a x )^\prime &= \dfrac{1}{x \ln a}

  \\

  ( \ln x )^\prime &= \dfrac{1}{x}

  \\

  ( a^x )^\prime &= x \ln a

  \\

  ( \sin x )^\prime &= \cos x

  \\

  ( \cos x )^\prime &= - \sin x

  \\

  ( \tan x )^\prime &= \dfrac{1}{\cos^2 x} = \sec^2 x

  \\

  ( \cot x )^\prime &= -\dfrac{1}{\sin^2 x} = - \csc^2 x

  \\

  ( \sec x )^\prime &= \dfrac{\sin x}{\cos^2 x} = \sec x \tan x

  \\

  ( \csc x )^\prime &= -\dfrac{\cos x}{\sin^2 x} = -\csc x \cot x

  \\

  ( \arcsin x )^\prime &= \dfrac{1}{\sqrt{1 - x^2}}

  \\

  ( \arccos x )^\prime &= -\dfrac{1}{\sqrt{1 - x^2}}

  \\

  ( \arctan x )^\prime &= \dfrac{1}{1 + x^2}

  \\

  ( \mathrm{arccot} \, x )^\prime &= -\dfrac{1}{1 + x^2}

  \\

  [ \ln ( x + \sqrt{x^2 - 1} )]^\prime &= \dfrac{1}{\sqrt{x^2 - 1}}

  \\

  [ \ln ( x + \sqrt{x^2 + 1} )]^\prime &= \dfrac{1}{\sqrt{x^2 + 1}}

\end{align*}
$$

---

$$
\begin{align*}

  ( u \pm v )^{( n )} &= u^{( n )} \pm v^{( n )}

  \\

  ( uv )^{( n )} &= \sum_{k = 0}^{n} \mathrm{C}_{n}^{k} u^{(n - k )} v^{( k )}

\end{align*}
$$

---

$$
\begin{align*}

  ( a^x )^{( n )} &= a^x ( \ln a )^n

  \\

  ( e^x )^{( n )} &= e^x

\end{align*}
$$

---

$$
\begin{align*}

  [ \sin ( kx ) ]^{( n )} &= k^n \sin ( kx + \dfrac{n}{2} \pi )

  \\

  [ \cos ( kx ) ]^{( n )} &= k^n \cos ( kx + \dfrac{n}{2} \pi )

\end{align*}
$$

---

$$
\begin{align*}

  ( \ln x )^{( n )} &= ( -1 )^{n - 1} \dfrac{( n - 1 ) !}{x^n} ( x > 0 )

  \\

  [ \ln ( x + 1 ) ]^{( n )} &= ( -1 )^{n-1} \dfrac{( n - 1 ) !}{( x + 1 )^{n}} ( x > -1 )

\end{align*}
$$

---

$$
\begin{align*}

  ( \dfrac{1}{x + a} )^{( n )} &= ( -1 )^n \dfrac{n !}{( x + a )^{n + 1}}

  \\

  [ ( x + x_0 )^m ]^{( n )} &= m ( m - 1) ( m - 2) \cdots ( m - n + 1 ) ( x + x_0 )^{m - n}

\end{align*}
$$
